ulib/LowStar.Regional.Instances.fst
@@ -35,7 +35,7 @@ val buffer_region_of:
 let buffer_region_of #a v =
   B.frameOf v
 
-val buffer_dummy: a:Type -> no_state_t -> Tot (B.buffer a)
+val buffer_dummy: a:Type -> unit -> Tot (B.buffer a)
 let buffer_dummy _ _ = B.null
 
 val buffer_r_inv:
@@ -88,7 +88,7 @@ let buffer_r_alloc_p #a v =
   True
 
 val buffer_r_alloc:
-  #a:Type -> ia:a -> len:UInt32.t{len > 0ul} -> no_state_t -> r:HST.erid ->
+  #a:Type -> ia:a -> len:UInt32.t{len > 0ul} -> unit -> r:HST.erid ->
   HST.ST (b:B.buffer a)
     (requires (fun h0 -> true))
     (ensures (fun h0 v h1 ->
@@ -105,7 +105,7 @@ let buffer_r_alloc #a ia len _ r =
 
 val buffer_r_free:
   #a:Type -> len:UInt32.t{len > 0ul} ->
-  no_state_t -> v:B.buffer a ->
+  unit -> v:B.buffer a ->
   HST.ST unit
     (requires (fun h0 -> buffer_r_inv len h0 v))
     (ensures (fun h0 _ h1 ->
@@ -114,7 +114,9 @@ let buffer_r_free #a len _ v =
   B.free v
 
 val buffer_copy:
-  #a:Type -> len:UInt32.t{len > 0ul} ->
+  #a:Type ->
+  len:UInt32.t{len > 0ul} ->
+  _:unit ->
   src:B.buffer a -> dst:B.buffer a ->
   HST.ST unit
     (requires (fun h0 ->
@@ -124,14 +126,14 @@ val buffer_copy:
       modifies (loc_all_regions_from false (buffer_region_of dst)) h0 h1 /\
       buffer_r_inv len h1 dst /\
       buffer_r_repr len h1 dst == buffer_r_repr len h0 src))
-let buffer_copy #a len src dst =
+let buffer_copy #a len _ src dst =
   B.blit src 0ul dst 0ul len
 
 val buffer_regional:
   #a:Type -> ia:a -> len:UInt32.t{len > 0ul} ->
-  regional no_state_t (B.buffer a)
+  regional unit (B.buffer a)
 let buffer_regional #a ia len =
-  Rgl no_state_val
+  Rgl ()
       (buffer_region_of #a)
       B.loc_buffer
       (buffer_dummy a)
@@ -149,44 +151,46 @@ let buffer_regional #a ia len =
 
 val buffer_copyable:
   #a:Type -> ia:a -> len:UInt32.t{len > 0ul} ->
-  copyable #no_state_t (B.buffer a) (buffer_regional ia len)
+  copyable #unit (B.buffer a) (buffer_regional ia len)
 let buffer_copyable #a ia len =
   Cpy (buffer_copy len)
 
 /// If `a` is regional, then `vector a` is also regional
 
+type vst (#a:Type0) (#rst:Type) = regional rst a
+
 val vector_region_of:
-  #a:Type -> #rg:regional no_state_t a -> v:rvector rg -> GTot HS.rid
-let vector_region_of #a #rg v = V.frameOf v
+  #a:Type0 -> #rst:Type -> #rg:vst -> v:rvector #a #rst rg -> GTot HS.rid
+let vector_region_of #a #rst #rg v = V.frameOf v
 
 val vector_dummy:
-  #a:Type -> rg:regional no_state_t a -> _:bool -> Tot (rvector rg)
-let vector_dummy #a _ rg = V.alloc_empty a
+  #a:Type0 -> #rst:Type -> s:vst -> Tot (rvector #a #rst s)
+let vector_dummy #a #_ _ = V.alloc_empty a
 
 val vector_r_inv:
-  #a:Type -> #rg:regional no_state_t a ->
-  h:HS.mem -> v:rvector rg -> GTot Type0
-let vector_r_inv #a #rg h v = RV.rv_inv h v
+  #a:Type0 -> #rst:Type -> #rg:vst ->
+  h:HS.mem -> v:rvector #a #rst rg -> GTot Type0
+let vector_r_inv #a #rst #rg h v = RV.rv_inv h v
 
 val vector_r_inv_reg:
-  #a:Type -> #rg:regional no_state_t a ->
-  h:HS.mem -> v:rvector rg ->
+  #a:Type0 -> #rst:Type -> #rg:vst ->
+  h:HS.mem -> v:rvector #a #rst rg ->
   Lemma (requires (vector_r_inv h v))
         (ensures (HS.live_region h (vector_region_of v)))
-let vector_r_inv_reg #a #rg h v = ()
+let vector_r_inv_reg #a #rst #rg h v = ()
 
-val vector_repr: #a:Type0 -> rg:regional no_state_t a -> Tot Type0
-let vector_repr #a rg = S.seq (Rgl?.repr rg)
+val vector_repr: #a:Type0 -> #rst:Type -> rg:vst #a #rst -> Tot Type0
+let vector_repr #a #rst rg = S.seq (Rgl?.repr rg)
 
 val vector_r_repr:
-  #a:Type -> #rg:regional no_state_t a ->
-  h:HS.mem -> v:rvector rg{vector_r_inv h v} ->
+  #a:Type0 -> #rst:Type -> #rg:vst ->
+  h:HS.mem -> v:rvector #a #rst rg{vector_r_inv h v} ->
   GTot (vector_repr rg)
-let vector_r_repr #a #rg h v = RV.as_seq h v
+let vector_r_repr #a #rst #rg h v = RV.as_seq h v
 
 val vector_r_sep:
-  #a:Type -> #rg:regional no_state_t a ->
-  v:rvector rg -> p:loc -> h0:HS.mem -> h1:HS.mem ->
+  #a:Type0 -> #rst:Type -> #rg:vst ->
+  v:rvector #a #rst rg -> p:loc -> h0:HS.mem -> h1:HS.mem ->
   Lemma (requires (vector_r_inv h0 v /\
                   loc_disjoint
                     (loc_all_regions_from false (vector_region_of v))
@@ -194,23 +198,23 @@ val vector_r_sep:
                   modifies p h0 h1))
         (ensures (vector_r_inv h1 v /\
                  vector_r_repr h0 v == vector_r_repr h1 v))
-let vector_r_sep #a #rg v p h0 h1 =
+let vector_r_sep #a #rst #rg v p h0 h1 =
   RV.rv_inv_preserved v p h0 h1;
   RV.as_seq_preserved v p h0 h1
 
 val vector_irepr:
-  #a:Type -> rg:regional no_state_t a -> Ghost.erased (vector_repr rg)
-let vector_irepr #a rg =
+  #a:Type0 -> #rst:Type -> rg:vst #a #rst -> Ghost.erased (vector_repr rg)
+let vector_irepr #a #rst rg =
   Ghost.hide S.empty
 
 val vector_r_alloc_p:
-  #a:Type -> #rg:regional no_state_t a -> v:rvector rg -> GTot Type0
-let vector_r_alloc_p #a #rg v =
+  #a:Type0 -> #rst:Type -> #rg:vst -> v:rvector #a #rst rg -> GTot Type0
+let vector_r_alloc_p #a #rst #rg v =
   V.size_of v = 0ul
 
 val vector_r_alloc:
-  #a:Type -> #rg:regional no_state_t a -> _:bool -> r:HST.erid ->
-  HST.ST (v:rvector rg)
+  #a:Type0 -> #rst:Type -> s:vst -> r:HST.erid ->
+  HST.ST (v:rvector #a #rst s)
     (requires (fun h0 -> true))
     (ensures (fun h0 v h1 ->
       Set.subset (Map.domain (HS.get_hmap h0))
@@ -220,33 +224,37 @@ val vector_r_alloc:
       vector_r_alloc_p v /\
       vector_r_inv h1 v /\
       vector_region_of v = r /\
-      vector_r_repr h1 v == Ghost.reveal (vector_irepr rg)))
-let vector_r_alloc #a #rg _ r =
+      vector_r_repr h1 v == Ghost.reveal (vector_irepr s)))
+let vector_r_alloc #a #rst s r =
   let nrid = HST.new_region r in
-  V.alloc_reserve 1ul (Rgl?.dummy rg (Rgl?.state rg)) r
+  V.alloc_reserve 1ul (rg_dummy s) r
 
 val vector_r_free:
-  #a:Type -> #rg:regional no_state_t a -> _:bool -> v:rvector rg ->
+  #a:Type0 -> #rst:Type -> s:vst #a #rst -> v:rvector #a #rst s ->
   HST.ST unit
     (requires (fun h0 -> vector_r_inv h0 v))
     (ensures (fun h0 _ h1 ->
       modifies (loc_all_regions_from false (vector_region_of v)) h0 h1))
-let vector_r_free #a #rg _ v =
-  RV.free v
+let vector_r_free #_ #_ _ v =
+  V.free v
 
 val vector_regional:
-  #a:Type -> rg:regional no_state_t a -> regional no_state_t (rvector rg)
-let vector_regional #a rg =
-  Rgl no_state_val
-      (vector_region_of #a #rg)
+  #a:Type0 -> #rst:Type -> rg:vst #a #rst -> regional (vst #a #rst) (rvector #a #rst rg)
+let vector_regional #a #rst rg =
+  [@inline_let] let f:((s:vst #a #rst{s==rg}) -> (v:rvector #a #rst s) -> HST.ST unit
+                    (requires (fun h0 -> vector_r_inv h0 v))
+                    (ensures (fun h0 _ h1 ->
+                         modifies (loc_all_regions_from false (vector_region_of v)) h0 h1))) = vector_r_free in
+  Rgl rg
+      (vector_region_of #a #rst #rg)
       V.loc_vector
-      (vector_dummy #a rg)
-      (vector_r_inv #a #rg)
-      (vector_r_inv_reg #a #rg)
+      (vector_dummy #a #rst)
+      (vector_r_inv #a #rst #rg)
+      (vector_r_inv_reg #a #rst #rg)
       (vector_repr #a rg)
-      (vector_r_repr #a #rg)
-      (vector_r_sep #a #rg)
+      (vector_r_repr #a #rst #rg)
+      (vector_r_sep #a #rst #rg)
       (vector_irepr #a rg)
-      (vector_r_alloc_p #a #rg)
-      (vector_r_alloc #a #rg)
-      (vector_r_free #a #rg)
+      (vector_r_alloc_p #a #rst #rg)
+      (vector_r_alloc #a #rst)
+      f
